{
 "cells": [
  {
   "cell_type": "markdown",
   "metadata": {},
   "source": [
    "# Solving a 1D Poisson equation with the finite element method (P2 elements)"
   ]
  },
  {
   "cell_type": "markdown",
   "metadata": {},
   "source": [
    "## General problem\n",
    "\n",
    "In this project we wish to sovle the following 1D Possion equation \n",
    "\n",
    "$$ -u''(x) = 2x-1, \\hspace{0.4cm} \\Omega = [0,1], \\hspace{0.3cm} u'(0) = C, \\hspace{0.3cm} u(1) = D, \\tag{1}$$\n",
    "\n",
    "where $C$ and $D$ are two scalar constants. We will use an uniform mesh consisting of $N_e$ elements, with P2 elements. This means that each element will contain 3 nodes, one local node and two global. The global nodes for each element will be shared among the elements, expect for the boundary elements which only share one node. The steplenght $h$ and mesh points $x_i$ is thus defined as\n",
    "\n",
    "$$h = \\frac{1}{2N_e}, \\qquad x_i = ih \\hspace{0.3cm} \\text{for } i=0,...,N$$\n",
    "\n",
    "with $N = (2N_e + 1)$ as the total number of nodes (both local and global nodes).\n",
    "\n",
    "## Task 1\n",
    "\n",
    "To derive the variational form of eq. (1) we can start from the general equation\n",
    "\n",
    "$$ -u''(x) = f(x). $$\n",
    "\n",
    "\n",
    "We wish to find a solution $u$ which lies in the vector space\n",
    "\n",
    "$$V = \\text{span}\\{\\psi_0,...,\\psi_N\\},$$\n",
    "\n",
    "meaning that $u$ can be expressed as a linear combination on the form\n",
    "\n",
    "$$u = \\sum_{j=0}^N c_j \\psi_j.$$\n",
    "\n",
    "In our current problem we have to account for the boundary condition $u(1) = D$ in the expression for $u$, but this is not necessary to include when deriving the variational form. We can rewrite eq. (1) as the abstract differential equation \n",
    "\n",
    "$$\\mathcal{L}(u) = u''(x) + f(x) = 0. \\tag{2}$$\n",
    "\n",
    "To formulate the variational form of eq. (1) we mulitply eq. (2) with an element from $V$ and integrate: \n",
    "\n",
    "$$ \\langle u''(x) + f(x), \\psi \\rangle \\hspace{0.5cm} \\forall \\psi \\in V \\tag{3}$$\n",
    "\n",
    "Here the inneproduct $\\langle f(x), g(x) \\rangle$ is defined as $\\int_{\\Omega} f(x)g(x) dx$. Rearranging eq. (3) we get\n",
    "\n",
    "$$ \\langle u''(x), \\psi \\rangle = - \\langle f(x), \\psi \\rangle. $$\n",
    "\n",
    "If we integrate the left-hand side by parts we obtain the variational form\n",
    "\n",
    "$$ \\langle u', \\psi' \\rangle = \\langle f, \\psi \\rangle + u'(1)\\psi(1) - C\\psi(0). \\tag{4}$$\n",
    "\n",
    "When solving eq. (1) the basis functions $\\psi_i$ for $i = 0,...,N$ are piecewise quadratic polynomials."
   ]
  },
  {
   "cell_type": "markdown",
   "metadata": {},
   "source": [
    "#### Specified variational form\n",
    "\n",
    "In our specific case we have the following expression for $u$:\n",
    "\n",
    "$$u = B(x) + \\sum_{j=0}^N c_j \\psi_j,$$\n",
    "\n",
    "with $B(x) = xD$ and the basis vectors $\\psi_j$ are Lagrange polynomials. We require that $\\psi_j(1) = 0$ since $u$ is specified at $x=1$, which gives us the following variational form\n",
    "\n",
    "$$ \\sum_{j=0}^N \\langle (B + c_j \\psi_j)', \\psi_i' \\rangle = \\langle 2x-1, \\psi_i \\rangle - C\\psi_i(0) $$\n",
    "\n",
    "$$ \\sum_{j=0}^N \\langle \\psi_j', \\psi_i' \\rangle c_j = \\langle 2x-1, \\psi_i \\rangle - C\\psi_i(0) - \\langle D, \\psi_i' \\rangle \\tag{5} $$\n",
    "\n",
    "Eq. (5) can be rewritten to a matrix equation with\n",
    "\n",
    "$$ \\sum_{j=0}^N A_{ij}c_j = \\sum_{j=0}^N \\langle \\psi_j', \\psi_i' \\rangle c_j,$$\n",
    "\n",
    "$$ b_i =  \\langle 2x-1, \\psi_i \\rangle - C\\psi_i(0) - \\langle D, \\psi_i' \\rangle \\tag{6}$$"
   ]
  },
  {
   "cell_type": "markdown",
   "metadata": {},
   "source": [
    "## Task 2\n",
    "\n",
    "The piecewise quadratic polynomials are found from the Lagrange polynomials,\n",
    "\n",
    "$$ \\psi_i = \\prod_{\\substack{j=0\\\\ j\\neq i}}^d \\frac{x-x_j}{x_i - x_j}, $$\n",
    "\n",
    "where $d$ is the number of nodes in element $i$. The entries in the element matrix $A$ is given by the inner product $A_{ij} = \\langle \\psi_j', \\psi_i' \\rangle$.\n",
    "\n",
    "* Leftmost element\n",
    "\n",
    "    The basis functions in $\\Omega^{(0)}$ are:\n",
    "    $$\\psi_0 = \\frac{(x-h)(x-2h)}{2h^2}$$\n",
    "    \n",
    "    $$\\psi_1 = - \\frac{x(x-2h)}{h^2} $$\n",
    "    \n",
    "    $$\\psi_2 = \\frac{x(x-h)}{2h^2} $$\n",
    "    \n",
    "    From SymPy we find the inner products, and thus the matrix elements:\n",
    "    $$ \\langle \\psi_0', \\psi_0' \\rangle = \\frac{13}{12h}, \\qquad \\langle \\psi_0', \\psi_1' \\rangle = -\\frac{7}{6h}, \\qquad \\langle \\psi_0', \\psi_2' \\rangle = \\frac{1}{6h}.$$\n",
    "    \n",
    "    $$ \\langle \\psi_1', \\psi_0' \\rangle = -\\frac{7}{6h}, \\qquad \\langle \\psi_1', \\psi_1' \\rangle = \\frac{4}{3h}, \\qquad \\langle \\psi_1', \\psi_2' \\rangle = -\\frac{7}{6h}.$$\n",
    "    \n",
    "    $$ \\langle \\psi_2', \\psi_0' \\rangle = \\frac{1}{6h}, \\qquad \\langle \\psi_2', \\psi_1' \\rangle = -\\frac{7}{6h}, \\qquad \\langle \\psi_2', \\psi_2' \\rangle = \\frac{13}{12h}.$$\n",
    "    \n",
    "    The right-hand side, given by eq. (6) is \n",
    "    \n",
    "    $$b_0 = \\frac{3}{4h} - \\frac{6h+1}{6h^2} + \\frac{1}{4h^2} - C + \\frac{3D}{2h} - \\frac{D}{2h^2}, $$\n",
    "    \n",
    "    $$b_1 = \\frac{1}{4h} - \\frac{2h+1}{6h^2} + \\frac{1}{4h^2} + \\frac{D}{h^2} - \\frac{2D}{h}, $$\n",
    "    \n",
    "    $$b_2 = \\frac{1}{4h} - \\frac{2h+1}{6h^2} + \\frac{1}{4h^2} + \\frac{D}{2h} - \\frac{D}{2h^2}. $$\n",
    "    \n",
    "* Rightmost element\n",
    "\n",
    "    The basis functions in $\\Omega^{(N_e)}$ are:\n",
    "    $$\\psi_{2N_e-2} = \\frac{(x-1 + h)(x-1)}{2h^2}$$\n",
    "    \n",
    "    $$\\psi_{2N_e-1} = - \\frac{(x-1+2h)(x-1)}{h^2} $$\n",
    "    \n",
    "    $$\\psi_{2N_e} = \\frac{(x-1+h)(x-1+2h)}{2h^2} $$\n",
    "    \n",
    "    From SymPy we find the inner products, and thus the matrix elements:\n",
    "    $$ \\langle \\psi_{2N_e-2}', \\psi_{2N_e-2}' \\rangle = \\frac{13}{12h}, \\qquad \\langle \\psi_{2N_e-2}', \\psi_{2N_e-1}' \\rangle = -\\frac{7}{6h}, \\qquad \\langle \\psi_{2N_e-2}', \\psi_{2N_e}' \\rangle = \\frac{1}{6h}.$$\n",
    "    \n",
    "    $$ \\langle \\psi_{2N_e-1}', \\psi_{2N_e-2}' \\rangle = -\\frac{7}{6h}, \\qquad \\langle \\psi_{2N_e-1}', \\psi_{2N_e-1}' \\rangle = \\frac{4}{3h}, \\qquad \\langle \\psi_{2N_e}', \\psi_{2N_e}' \\rangle = -\\frac{7}{6h}.$$\n",
    "    \n",
    "    $$ \\langle \\psi_{2N_e}', \\psi_{2N_e-2}' \\rangle = \\frac{1}{6h}, \\qquad \\langle \\psi_{2N_e}', \\psi_{2N_e-1}' \\rangle = -\\frac{7}{6h}, \\qquad \\langle \\psi_{2N_e}', \\psi_{2N_e}' \\rangle = \\frac{13}{12h}.$$\n",
    "    \n",
    "    The right-hand side, given by eq. (6) is \n",
    "    \n",
    "    $$b_{2N_e-2} = \\frac{(h-1)}{12h^2} - \\frac{C(1-h)}{2h^2} - \\frac{D(h-1)}{2h^2}, $$\n",
    "    \n",
    "    $$b_{2N_e-1} = \\frac{(3h-1)}{12h^2} - \\frac{C(2h-1)}{h^2} - \\frac{D(1-2h)}{h^2}, $$\n",
    "    \n",
    "    $$b_{2N_e} = \\frac{(3h-1)}{12h^2} - \\frac{C(2h-1)}{h^2} + \\frac{D(3h-1)}{2h^2}. $$\n"
   ]
  },
  {
   "cell_type": "code",
   "execution_count": null,
   "metadata": {},
   "outputs": [],
   "source": []
  }
 ],
 "metadata": {
  "kernelspec": {
   "display_name": "Python 3",
   "language": "python",
   "name": "python3"
  },
  "language_info": {
   "codemirror_mode": {
    "name": "ipython",
    "version": 3
   },
   "file_extension": ".py",
   "mimetype": "text/x-python",
   "name": "python",
   "nbconvert_exporter": "python",
   "pygments_lexer": "ipython3",
   "version": "3.8.5"
  }
 },
 "nbformat": 4,
 "nbformat_minor": 4
}
